More work in RefinedHeap.v

RefinedHeap.v
@@ -23,16 +23,12 @@ Variable Zero : Word8.
 Definition MemoryBlock := MemoryBlock Word8.
 Definition HeapSpec := @HeapSpec Word8.
 
+Section MemoryBlock.
+
 Record MemoryBlockC := {
   memCSize : N;
   memCData : M.t Word8
 }.
-
-Require Import
-  Fiat.ADT
-  Fiat.ADTNotation
-  Fiat.ADTRefinement
-  Fiat.ADTRefinement.BuildADTRefinements.
 
 Definition MemoryBlock_AbsR (o : MemoryBlock) (n : MemoryBlockC) : Prop :=
   memSize o = memCSize n /\
@@ -47,38 +43,94 @@ Proof.
   exact (Empty_SetMap_AbsR _).
 Qed.
 
-Lemma free_test_proper : forall n,
-  Proper (eq ==> eq ==> eq)
-    (fun (addr : M.key) (blk : MemoryBlockC) => addr + memCSize blk <=? n).
+End MemoryBlock.
+
+Require Import
+  Fiat.ADT
+  Fiat.ADTNotation
+  Fiat.ADTRefinement
+  Fiat.ADTRefinement.BuildADTRefinements.
+
+Definition within_allocated_mem (n : N) :=
+  fun (addr : M.key) (blk : MemoryBlockC) => addr + memCSize blk <=? n.
+
+Lemma within_allocated_mem_Proper : forall n,
+  Proper (eq ==> eq ==> eq) (within_allocated_mem n).
 Proof.
   unfold Proper, respectful; intros.
   subst; reflexivity.
 Qed.
 
-Hint Resolve free_test_proper.
+Lemma within_allocated_mem_add : forall n x k e,
+  within_allocated_mem n k e
+    -> 0 < x
+    -> within_allocated_mem (n + x) k e.
+Proof.
+  unfold within_allocated_mem; intros.
+  undecide.
+  apply Nle_add_plus; trivial.
+Qed.
 
-Ltac remove_dependency :=
-  repeat
-    match goal with
-      | [ |- refine (_ <- `(_|_) <- ret _;
-                          ret _;
-                     _) _ ] =>
-        rewrite refine_bind_dep_ret
-      | [ |- refine (_ <- `(_|_) <- _;
-                          ret _;
-                     _) _ ] =>
-        rewrite refine_bind_dep_bind_ret; simpl
-      | [ |- refine (`(_|_) <- _;
-                     _) _ ] =>
-        rewrite refine_bind_dep_ignore
-    end.
+Lemma within_allocated_mem_at_end : forall n x d,
+   within_allocated_mem (n + x) n {| memCSize := x; memCData := d |}.
+Proof.
+  unfold within_allocated_mem; simpl; intros.
+  apply N.leb_refl.
+Qed.
+
+Hint Resolve within_allocated_mem_Proper.
 
 Definition Heap_AbsR
            (or : { r : Rep HeapSpec
                  | ADTInduction.fromADT HeapSpec r})
            (nr : N * M.t MemoryBlockC) : Prop :=
   SetMap_AbsR (` or) (snd nr) MemoryBlock_AbsR /\
-  P.for_all (fun addr blk => addr + memCSize blk <=? fst nr) (snd nr).
+  P.for_all (within_allocated_mem (fst nr)) (snd nr).
+
+Lemma find_found_block
+      {r_o r_n}
+      (AbsR : Heap_AbsR r_o r_n)
+      addr' len' data' :
+  found_block_at_base addr' len' data' (` r_o)
+    -> exists cdata',
+        SetMap_AbsR data' cdata' eq /\
+        M.find addr' (snd r_n)
+          = Some {| memCSize := len'; memCData := cdata' |}.
+Proof.
+  unfold found_block_at_base; intros.
+  destruct AbsR.
+  destruct (H0 addr'); clear H0.
+  destruct (H2 _ H) as [blk [? ?]]; clear H H2 H3.
+  exists (memCData blk).
+  destruct H4; simpl in *; subst.
+  destruct blk; simpl in *; auto.
+Qed.
+
+Lemma Heap_AbsR_outside_mem
+      {r_o r_n}
+      (AbsR : Heap_AbsR r_o r_n)
+      (d : {len : N | 0 < len}) :
+  forall addr' len' data',
+    found_block_at_base addr' len' data' (` r_o)
+      -> ~ overlaps addr' len' (fst r_n) (` d).
+Proof.
+  destruct AbsR; intros.
+  destruct d; simpl in *.
+  eapply find_found_block in H1; eauto;
+  [| split; [exact H|assumption] ].
+  destruct H1 as [cdata' [? ?]].
+  eapply P.for_all_iff
+    with (k:=addr')
+         (e:={| memCSize := len'
+              ; memCData := cdata' |}) in H0; eauto.
+    unfold within_allocated_mem in H0; simpl in H0.
+    unfold overlaps.
+    clear -H0 l.
+    undecide.
+    nomega.
+  apply F.find_mapsto_iff.
+  assumption.
+Qed.
 
 Ltac AbsR_prep :=
   repeat
@@ -106,8 +158,8 @@ Proof.
       finish honing.
 
     AbsR_prep.
-    - exact (Empty_SetMap_AbsR _).
-    - eapply E.for_all_empty; auto.
+    - apply Empty_SetMap_AbsR; trivial.
+    - apply E.for_all_empty; trivial.
   }
 
   refine method allocS.
@@ -118,8 +170,7 @@ Proof.
 
     refine pick val (fst r_n).
       Focus 2.
-      intros.
-      admit.
+      apply Heap_AbsR_outside_mem; trivial.
 
     simplify with monad laws; simpl.
     refine pick val (fst r_n + proj1_sig d,
@@ -130,15 +181,13 @@ Proof.
       finish honing.
 
     AbsR_prep.
-    - apply Update_SetMap_AbsR; auto.
-      exact (Empty_MemoryBlock_AbsR _).
-    - apply E.for_all_add; simpl; auto.
-        eapply for_all_impl; eauto; simpl; intros.
+    - apply Update_SetMap_AbsR; trivial.
+      apply Empty_MemoryBlock_AbsR; trivial.
+    - apply E.for_all_add; trivial.
+        eapply E.for_all_impl; eauto; intros.
         destruct d; simpl.
-        clear -l H2.
-        undecide.
-        apply Nle_add_plus; trivial.
-      apply N.leb_refl.
+        apply within_allocated_mem_add; trivial.
+      apply within_allocated_mem_at_end.
   }
 
   refine method freeS.
@@ -152,12 +201,16 @@ Proof.
       finish honing.
 
     AbsR_prep.
-    - admit.
-    - apply for_all_remove; auto.
+    - apply Remove_SetMap_AbsR; trivial.
+    - apply E.for_all_remove; trivial.
   }
 
   refine method reallocS.
   {
+    unfold Heap_AbsR, realloc, find_free_block.
+    remove_dependency.
+    simplify with monad laws; simpl.
+
     admit.
   }
 
@@ -179,6 +232,39 @@ Proof.
             Else Zero
        Else Zero).
       Focus 2.
+      simpl; intros; subst.
+      destruct H1.
+      apply (@find_found_block _ r_n) in H1; trivial.
+      destruct H1 as [cdata' [? ?]].
+      apply F.find_mapsto_iff in H4.
+      apply F.elements_mapsto_iff in H4.
+      destruct (M.elements (elt:=MemoryBlockC) (snd r_n)).
+        inversion H4.
+      apply SetoidList.InA_cons in H4.
+      destruct H4; simpl.
+        destruct H4.
+        simpl in *; subst.
+        rewrite <- H5; simpl.
+        unfold within in H3.
+        decisions.
+          simpl.
+          destruct (H1 (d - fst p)); clear H1 H6.
+          destruct (H4 _ H2); clear H4 H2.
+          rewrite <- H5; simpl.
+          destruct H1; subst.
+          setoid_rewrite H1.
+          reflexivity.
+        apply Bool.andb_false_iff in Heqe.
+        destruct H3.
+        destruct Heqe;
+        undecide;
+        apply N.nle_gt in H6;
+        firstorder.
+      apply P.of_list_1 in H4.
+      eapply F.elements_mapsto_iff in H4.
+      decisions.
+        simpl.
+        admit.
       admit.
 
     simplify with monad laws; simpl.
@@ -194,6 +280,7 @@ Proof.
     unfold poke, set_address.
     remove_dependency.
     simplify with monad laws; simpl.
+
     refine pick val
       (fst r_n,
        M.mapi (fun addr blk =>
@@ -206,19 +293,26 @@ Proof.
       finish honing.
 
     AbsR_prep.
-    - apply Map_SetMap_AbsR; auto.
-      intros.
+    - apply Map_SetMap_AbsR; auto; intros.
       admit.
     - admit.
   }
 
   refine method memcpyS.
   {
+    unfold memcpy.
+    remove_dependency.
+    simplify with monad laws; simpl.
+
     admit.
   }
 
   refine method memsetS.
   {
+    unfold memset.
+    remove_dependency.
+    simplify with monad laws; simpl.
+
     admit.
   }
 
